src/num/extra_theories/dividesScript.sml
@@ -1,7 +1,8 @@
 structure dividesScript =
 struct
 
-open HolKernel Parse boolLib BasicProvers arithmeticTheory simpLib SingleStep;
+open HolKernel Parse boolLib BasicProvers arithmeticTheory 
+     simpLib SingleStep metisLib;
 
 val arith_ss = simpLib.++(bool_ss, numSimps.ARITH_ss)
 
@@ -117,6 +118,34 @@ val NOT_PRIME_1 = Q.store_thm
   `~prime 1`,
   ARW[prime_def, DIVIDES_LE]);
 val _ = export_rewrites ["NOT_PRIME_1"]
+
+
+(*---------------------------------------------------------------------------*)
+(* Directly computable version of divides                                    *)
+(*---------------------------------------------------------------------------*)
+
+val compute_divides = Q.store_thm
+("compute_divides",
+ `!a b. divides a b = 
+        if a=0 then (b=0) else
+        if a=1 then T else 
+        if b=0 then T else
+        (b MOD a = 0)`,
+  RW_TAC arith_ss [divides_def] 
+   THEN EQ_TAC 
+   THEN RW_TAC arith_ss [] THENL
+   [Cases_on `q` THENL 
+     [RW_TAC arith_ss [],
+      `0<a` by RW_TAC arith_ss [] THEN 
+      METIS_TAC [MOD_MULT, MULT_SYM, ADD_CLAUSES]],
+    Q.EXISTS_TAC `b` THEN RW_TAC arith_ss [],
+    Q.EXISTS_TAC `0` THEN RW_TAC arith_ss [],
+    `0<a` by RW_TAC arith_ss [] THEN
+     let val MOD_P_inst = BETA_RULE (Q.SPECL[`\x. (x = 0)`,`b`,`a`] MOD_P)
+     in METIS_TAC [MOD_P_inst,MULT_SYM, ADD_CLAUSES]
+     end]);
+
+val _ = computeLib.add_persistent_funs [("compute_divides",compute_divides)];
 
 val _ = export_theory();
 
